Smaller diff, keep the 'run' in line with other stuff

Manual/VCGen.lean
@@ -447,19 +447,19 @@ set_option mvcgen.warning false
 The single-field structure {name}`Identity` acts like the identity monad {name}`Id`. It has a {name}`WP` instance, but no {name}`WPMonad` instance:
 ```lean
 structure Identity (α : Type u) where
-  value : α
+  run : α
 
 variable {α : Type u}
 
 instance : Monad Identity where
   pure x := ⟨x⟩
-  bind x f := f x.value
+  bind x f := f x.run
 
 instance : WP Identity .pure where
-  wp x := PredTrans.pure x.value
+  wp x := PredTrans.pure x.run
 
 theorem Identity.of_wp_run_eq {x : α} {prog : Identity α}
-    (h : Identity.value prog = x) (P : α → Prop) :
+    (h : Identity.run prog = x) (P : α → Prop) :
     (⊢ₛ wp⟦prog⟧ (⇓ a => ⟨P a⟩)) → P x := by
   simp_all [WP.wp, ← h]
 ```
@@ -486,8 +486,8 @@ It is correct if it is equal to {name}`List.reverse`.
 However, {tactic}`mvcgen` does not make the goal easier to prove:
 ```lean +error -keep (name := noInst)
 theorem rev_correct :
-    (rev xs).value = xs.reverse := by
-  generalize h : (rev xs).value = x
+    (rev xs).run = xs.reverse := by
+  generalize h : (rev xs).run = x
   apply Identity.of_wp_run_eq h
   mvcgen [rev]
 ```
@@ -496,7 +496,7 @@ unsolved goals
 case vc1
 α✝ : Type u_1
 xs x : List α✝
-h : (rev xs).value = x
+h : (rev xs).run = x
 out✝ : List α✝ := []
 ⊢ (wp⟦do
       let __s ← forIn xs out✝ fun x __s => pure (ForInStep.yield (x :: __s))
@@ -513,8 +513,8 @@ instance : WPMonad Identity .pure where
 With this instance, and a suitable invariant, {tactic}`mvcgen` and {tactic}`grind` can prove the theorem.
 ```lean
 theorem rev_correct :
-    (rev xs).value = xs.reverse := by
-  generalize h : (rev xs).value = x
+    (rev xs).run = xs.reverse := by
+  generalize h : (rev xs).run = x
   apply Identity.of_wp_run_eq h
   simp only [rev]
   mvcgen invariants
